src/ExpandWhens.v
@@ -1,0 +1,1450 @@
+From Coq Require Import BinNat ZArith Lia.
+From mathcomp Require Import ssreflect ssrbool eqtype seq fintype ssrnat div ssrfun.
+From simplssrlib Require Import SsrOrder Var FMaps.
+From firrtl Require Import Firrtl Env HiEnv HiFirrtl.
+
+Section ExpandWhens.
+
+  (* a type to indicate connects *)
+Inductive def_expr : Type :=
+  | D_undefined (* declared but not connected, no "is invalid" statement *)
+  | D_invalidated (* declared but not connected, there is a "is invalid" statement *)
+  | D_fexpr : HiFP.hfexpr -> def_expr (* declared and connected *)
+  .
+
+(* equality of def_expr is decidable [because equality of hfexpr is decidable] *)
+Lemma def_expr_eq_dec : forall {x y : def_expr}, {x = y} + {x <> y}.
+  Proof.
+  decide equality.
+  apply hfexpr_eq_dec.
+Qed.
+
+Definition def_expr_eqn (x y : def_expr) : bool :=
+  match x, y with
+  | D_undefined, D_undefined => true
+  | D_invalidated, D_invalidated => true
+  | D_fexpr expr1, D_fexpr expr2 => expr1 == expr2
+  | _, _ => false
+  end.
+
+Lemma def_expr_eqP : Equality.axiom def_expr_eqn.
+Proof.
+  unfold Equality.axiom, def_expr_eqn.
+  intros ; induction x, y ; try (apply ReflectF ; discriminate) ; try (apply ReflectT ; reflexivity).
+  case Eq: (h == h0).
+  all: move /hfexpr_eqP : Eq => Eq.
+  apply ReflectT ; replace h0 with h ; reflexivity.
+  apply ReflectF ; injection ; apply Eq.
+Qed.
+
+Canonical def_expr_eqMixin := EqMixin def_expr_eqP.
+Canonical def_expr_eqType := Eval hnf in EqType def_expr def_expr_eqMixin.
+
+Definition helper_tf (c : HiFP.hfexpr) (true_expr : option def_expr) (false_expr : option def_expr) : option def_expr := (* ? *)
+  match true_expr, false_expr with
+  | None, None => None
+  | Some (D_fexpr t), Some (D_fexpr f) => (*if t == f then true_expr 
+                                      else*) Some (D_fexpr (Emux c t f)) 
+  | Some D_invalidated, Some (D_fexpr f) => false_expr
+  | Some (D_fexpr t), Some D_invalidated => true_expr
+  | _,_ => true_expr (* impossible? *)
+  end.
+
+(*Definition combine_branches (c : HiFP.hfexpr) (true_branch : (HiFP.hfstmt_seq * CEP.t def_expr)) (false_branch: (HiFP.hfstmt_seq * CEP.t def_expr)) : (HiFP.hfstmt_seq * CEP.t def_expr) :=
+  let combined_cm := CEP.map2 (helper_tf c) (snd true_branch) (snd false_branch) (* CE.map2 for what? *)
+   in (Qcat (fst true_branch) (fst false_branch), combined_cm). (* 直接Qcat？如果有重复定义 *)
+
+Definition init_ref (r : pvar) (type : ftype) (cm : CEP.t def_expr) : CEP.t def_expr :=
+  match type with
+  | Gtyp _ => CEP.add r D_undefined cm
+  | _ => cm (* should be changed in expand connects *)
+  end.
+
+Definition init_register (r : pvar) (type : ftype) (cm : CEP.t def_expr) : CEP.t def_expr :=
+   match type with
+   | Gtyp _ => CEP.add r (D_fexpr (Eref (Eid r))) cm
+   | _ => cm
+   end.
+
+Definition init_inv (r : pvar) (cm : CEP.t def_expr) : CEP.t def_expr :=
+  CEP.add r D_invalidated cm.
+
+Definition init_inst (r : pvar) (mv: pvar) (ce_other_modules : CEP.env) (cm : CEP.t def_expr) : CEP.t def_expr :=
+   match CEP.find mv ce_other_modules with
+   | Some (HiFP.aggr_typ t, Instanceof) => init_ref r t cm
+   (* CEP.find v1 ce' = Some (fst (CEP.vtyp v2 ce), Instanceof) -> *)
+   | _ => cm (* wrong initialization *)
+   end.
+
+   old version
+
+ Fixpoint expandBranch_fun (ss : HiFP.hfstmt_seq) (ce_other_modules : CEP.env) (hseq_result : HiFP.hfstmt_seq) (cm_result : CEP.t def_expr) : (HiFP.hfstmt_seq * CEP.t def_expr) :=
+  (* ss : statement seq going to be expanded 
+     ce_other_modules : type information for ports of other modules, used in inst case
+     hseq_result : declaration statement in ss, including those in branches
+     cm_result : rhs expr map for every var that is connected to, also solving last connecting*)
+  match ss with
+  | Qnil => (hseq_result, cm_result)
+  | Qcons s st => let (new_hseq, new_cm) := 
+    match s with
+    | Sskip => (hseq_result, cm_result) (* no translation needed *)
+    | Swire v type => let cm_wire := init_ref v type cm_result
+                      in (Qcons s hseq_result, cm_wire)
+    | Sreg v r => let cm_reg := init_register v (type r) cm_result
+                  in (Qcons s hseq_result, cm_reg)
+    | Smem v m => let cm_mem := cm_result
+                  in (Qcons s hseq_result, cm_mem) (* TBD *)
+    | Sinvalid (Eid r) => let cm_inv := init_inv r cm_result
+                    in (hseq_result, cm_inv)
+    | Sinst v v0 => let cm_inst := cm_result 
+                    in (Qcons s hseq_result, cm_inst) (* TBD *)
+    | Snode v e => (Qcons s hseq_result, cm_result)
+    | Sfcnct (Eid r) e2 => let cm_cnct := CEP.add r (D_fexpr e2) cm_result
+                            in (hseq_result, cm_cnct)
+    | Swhen c s1 s2 => let cm_true := expandBranch_fun s1 ce_other_modules hseq_result cm_result in
+                       let cm_false := expandBranch_fun s2 ce_other_modules (Qnil ProdVarOrder.T) cm_result in
+                       combine_branches c cm_true cm_false
+    | _ => (hseq_result, cm_result) (* subindex subaccess subfield don't exist *)
+    end in expandBranch_fun st ce_other_modules new_hseq new_cm
+  end.*)
+
+Fixpoint expandBranch_fun (s : HiFP.hfstmt) (hseq_result : option HiFP.hfstmt_seq) (cm_result : CEP.t def_expr) : (option HiFP.hfstmt_seq * CEP.t def_expr) :=
+  (* ss : statement seq going to be expanded 
+     ce_other_modules : type information for ports of other modules, used in inst case
+     hseq_result : declaration statement in ss, including those in branches
+     cm_result : rhs expr map for every var that is connected to, also solving last connecting*)
+  match s with
+  | Sskip => (hseq_result, cm_result)
+  | Swire v type => let new_seq := match hseq_result with
+                    | None => None
+                    | Some hseq_result => if (Qin s hseq_result) then None else Some (Qcons s hseq_result)
+                    end in
+                    let cm_wire := CEP.add v D_undefined cm_result
+                    in (new_seq, cm_wire)
+  | Sreg v r => let new_seq := match hseq_result with
+                | None => None
+                | Some hseq_result => if (Qin s hseq_result) then None else Some (Qcons s hseq_result)
+                end in
+                let cm_reg := CEP.add v (D_fexpr (Eref (Eid v))) cm_result
+                in (new_seq, cm_reg)
+  | Smem v m => let new_seq := match hseq_result with
+                | None => None
+                | Some hseq_result => if (Qin s hseq_result) then None else Some (Qcons s hseq_result)
+                end in
+                let cm_mem := CEP.add v D_undefined cm_result
+                in (new_seq, cm_mem) (* TBD *)
+  | Sinvalid (Eid r) => let cm_inv := CEP.add r D_invalidated cm_result
+                        in (hseq_result, cm_inv)
+  | Sinst v v0 => let new_seq := match hseq_result with
+                  | None => None
+                  | Some hseq_result => if (Qin s hseq_result) then None else Some (Qcons s hseq_result)
+                  end in
+                  let cm_inst := CEP.add v D_undefined cm_result
+                  in (new_seq, cm_inst) (* TBD *)
+  | Snode v e => let new_seq := match hseq_result with
+                | None => None
+                | Some hseq_result => if (Qin s hseq_result) then None else Some (Qcons s hseq_result)
+                end in (new_seq, cm_result)
+  | Sfcnct (Eid r) e2 => let cm_cnct := CEP.add r (D_fexpr e2) cm_result
+                          in (hseq_result, cm_cnct)
+  | Swhen c s1 s2 => (*let (new_seq0, cm_true) := expandBranch_funs s1 hseq_result cm_result in*)
+                     (*let (new_seq, cm_false) := expandBranch_funs s2 (fst (expandBranch_funs s1 hseq_result cm_result)) cm_result in*)
+                     ((fst (expandBranch_funs s2 (fst (expandBranch_funs s1 hseq_result cm_result)) cm_result)),
+                      CEP.map2 (helper_tf c) (snd (expandBranch_funs s1 hseq_result cm_result)) (snd (expandBranch_funs s2 (fst (expandBranch_funs s1 hseq_result cm_result)) cm_result)))
+  | _ => (hseq_result, cm_result) 
+  end
+with expandBranch_funs (ss : HiFP.hfstmt_seq) (hseq_result : option HiFP.hfstmt_seq) (cm_result : CEP.t def_expr) : (option HiFP.hfstmt_seq * CEP.t def_expr) :=
+  match ss with
+  | Qnil => (hseq_result, cm_result)
+  | Qcons s stl => (*let (new_hseq, new_cm) := expandBranch_fun s hseq_result cm_result in *)
+                   expandBranch_funs stl (fst (expandBranch_fun s hseq_result cm_result)) (snd (expandBranch_fun s hseq_result cm_result))
+  end.
+
+Definition unfold_cm (cml : seq (pvar * def_expr)) sts := 
+  match cml with 
+  | nil => sts
+  | e :: es => match e with
+              | (v, D_fexpr tempe) => Qcons (Sfcnct (Eid v) tempe) sts
+              | (v, D_invalidated) => Qcons (Sinvalid (Eid v)) sts
+              | _ => sts (* D_undefined 未被连接error *)
+              end
+  end.
+
+Definition expandwhens_ss (dclseq : HiFP.hfstmt_seq) (cm : CEP.t def_expr) : HiFP.hfstmt_seq :=
+  let newcncts := unfold_cm (CEP.elements cm) (Qnil ProdVarOrder.T) in
+  (Qcat newcncts dclseq). (* rev *)
+
+  (* Definition cm_true := expandBranch_fun (Qcons est (Qnil ProdVarOrder.T)) ce0 (Qnil ProdVarOrder.T) (CEP.empty def_expr).
+  Definition cm_false := expandBranch_fun (Qcons esf (Qnil ProdVarOrder.T)) ce0 (Qnil ProdVarOrder.T) (CEP.empty def_expr).
+  Compute (CEP.find p1 (snd cm_true)).
+  Compute (CEP.find p1 (snd cm_false)).
+  Definition cm_new := CEP.map2 (helper_tf ec0) (snd cm_true) (snd cm_false).
+  Compute (CEP.find p1 cm_new). 
+
+  Definition ss := fst (expandBranch_fun ess ce0 (Qnil ProdVarOrder.T) (CEP.empty def_expr)).
+  Definition cm1 := snd (expandBranch_fun ess ce0 (Qnil ProdVarOrder.T) (CEP.empty def_expr)).
+  Compute (ss). *)
+ 
+(* another case: true branch == false branch 需要化简，没有mux *)
+
+(* Proof of declarations *)
+Fixpoint expandBranch_declaration (init_decl_map : CEP.env) (s : HiFP.hfstmt) (ce : CEP.env) : CEP.env :=
+  match s with
+  | Sskip => init_decl_map
+  | Swire v type => match (CEP.find v init_decl_map) with
+                    | None => CEP.add v (HiFP.aggr_typ type, Wire) init_decl_map
+                    | Some _ => CEP.remove v init_decl_map
+                    end
+  | Sreg v r => match (CEP.find v init_decl_map) with
+                | None => CEP.add v (HiFP.reg_typ r, Register) init_decl_map
+                | Some _ => CEP.remove v init_decl_map
+                end
+  | Smem v m => match (CEP.find v init_decl_map) with
+                | None => CEP.add v (HiFP.mem_typ m, Memory) init_decl_map
+                | Some _ => CEP.remove v init_decl_map
+                end
+  | Sinst v v0 => match (CEP.find v init_decl_map) with
+                | None => CEP.add v (fst (CEP.vtyp v0 ce), Instanceof) init_decl_map
+                | Some _ => CEP.remove v init_decl_map
+                end
+  | Snode v e => match (CEP.find v init_decl_map) with
+                | None => CEP.add v (HiFP.aggr_typ (HiFP.type_of_hfexpr e ce), Node) init_decl_map
+                | Some _ => CEP.remove v init_decl_map
+                end
+  | Swhen c s1 s2 => let new_decl_map := expandBranch_declarations init_decl_map s1 ce in
+                      expandBranch_declarations new_decl_map s2 ce
+  | _ => init_decl_map
+  end
+with expandBranch_declarations (init_decl_map : CEP.env) (ss : HiFP.hfstmt_seq) (ce : CEP.env) : CEP.env :=
+  match ss with
+  | Qnil => init_decl_map
+  | Qcons s stl => let newmap := expandBranch_declaration init_decl_map s ce in 
+                   expandBranch_declarations newmap stl ce
+  end.
+(* old version
+  match ss with
+  | Qnil => init_decl_map
+  | Qcons s st => let new_decl_map := (match s with
+                  | Sskip => init_decl_map
+                  | Swire v type => CEP.add v (HiFP.aggr_typ type, Wire) init_decl_map
+                  | Sreg v r => CEP.add v (HiFP.reg_typ r, Register) init_decl_map
+                  | Smem v m => CEP.add v (HiFP.mem_typ m, Memory) init_decl_map
+                  | Sinst v v0 => CEP.add v (fst (CEP.vtyp v0 ce), Instanceof) init_decl_map
+                  | Snode v e => CEP.add v (HiFP.aggr_typ (HiFP.type_of_hfexpr e ce), Node) init_decl_map
+                  | Swhen c s1 s2 => let new_decl_map := expandBranch_declarations init_decl_map s1 ce in
+                                      expandBranch_declarations new_decl_map s2 ce
+                  | _ => init_decl_map
+                  end) in
+                  expandBranch_declarations new_decl_map st ce
+  end.
+*)
+
+Inductive expandBranch_declaration_stmt : HiFP.hfstmt -> HiFP.hfstmt_seq -> CEP.env -> CEP.env -> Prop :=
+  | ExpandBranch_declaration_skip seq_init ce ce':
+      expandBranch_declaration_stmt (HiFP.sskip) seq_init ce ce'
+  | ExpandBranch_declaration_wire v t seq_init ce ce' :
+      forall envce, 
+      CEP.Equal (expandBranch_declarations (expandBranch_declaration ce (Swire v t) envce) seq_init envce) ce' -> 
+      expandBranch_declaration_stmt (Swire v t) seq_init ce ce'
+  | ExpandBranch_declaration_reg v r seq_init ce ce' :
+      forall envce, 
+      CEP.Equal (expandBranch_declarations (expandBranch_declaration ce (Sreg v r) envce) seq_init envce) ce' -> 
+      expandBranch_declaration_stmt (Sreg v r) seq_init ce ce'
+  | ExpandBranch_declaration_inst v1 v2 seq_init ce ce' :
+      forall envce, 
+      CEP.Equal (expandBranch_declarations (expandBranch_declaration ce (Sinst v1 v2) envce) seq_init envce) ce' -> 
+      expandBranch_declaration_stmt (Sinst v1 v2) seq_init ce ce'
+  | ExpandBranch_declaration_node v e seq_init ce ce' :
+      forall envce, 
+      CEP.Equal (expandBranch_declarations (expandBranch_declaration ce (Snode v e) envce) seq_init envce) ce' -> 
+      expandBranch_declaration_stmt (Snode v e) seq_init ce ce'
+  | ExpandBranch_declaration_mem v m seq_init ce ce' :
+      forall envce, 
+      CEP.Equal (expandBranch_declarations (expandBranch_declaration ce (Smem v m) envce) seq_init envce) ce' -> 
+      expandBranch_declaration_stmt (Smem v m) seq_init ce ce'
+  | ExpandBranch_declaration_invalid v seq_init ce ce' :
+      forall envce, 
+      CEP.Equal (expandBranch_declarations (expandBranch_declaration ce (Sinvalid v) envce) seq_init envce) ce' -> 
+      expandBranch_declaration_stmt (Sinvalid v) seq_init ce ce'
+  | ExpandBranch_declaration_fcnct v e seq_init ce ce' :
+      forall envce, 
+      CEP.Equal (expandBranch_declarations (expandBranch_declaration ce (Sfcnct v e) envce) seq_init envce) ce' -> 
+      expandBranch_declaration_stmt (Sfcnct v e) seq_init ce ce'
+  | ExpandBranch_declaration_when c s1 s2 seq_init seq_init' ce ce' ce'' :
+      expandBranch_declaration_stmts s1 seq_init ce ce' ->
+      expandBranch_declaration_stmts s2 seq_init' ce ce'' ->
+      expandBranch_declaration_stmt (Swhen c s1 s2) seq_init ce ce''
+with expandBranch_declaration_stmts : HiFP.hfstmt_seq -> HiFP.hfstmt_seq -> CEP.env -> CEP.env -> Prop := 
+  | ExpandBranch_declarations_nil seq_init ce ce' :
+      expandBranch_declaration_stmts HiFP.qnil seq_init ce ce'
+  | ExpandBranch_declarations_con s ss seq_init seq_init' ce ce' ce'' :
+      expandBranch_declaration_stmt s seq_init ce ce' ->
+      expandBranch_declaration_stmts ss seq_init' ce ce'' ->
+      expandBranch_declaration_stmts (Qcons s ss) seq_init ce ce''.
+
+(* old version lemma
+
+Lemma cons_expandBranch_declarations (ss : HiFP.hfstmt_seq):
+forall (seq_init : HiFP.hfstmt_seq) (seq_result : HiFP.hfstmt_seq) (cm_result : CEP.t def_expr),
+  (expandBranch_funs ss (Some (Qnil ProdVarOrder.T)) cm_result).1 = Some seq_result ->
+  (expandBranch_funs ss (Some seq_init) cm_result).1 = Some (Qcat seq_result seq_init).
+Proof. 
+  Admitted.
+
+Lemma cat_expandBranch_delarations ss0 ss1:
+  forall (ce: CEP.env) (cm : CEP.env),
+  expandBranch_declarations cm (Qcat ss0 ss1) ce = expandBranch_declarations (expandBranch_declarations cm ss1 ce) ss0 ce.
+Proof.
+  Admitted.
+
+Definition well_defined_stmt s cm seq_init : Prop :=
+  match (expandBranch_fun s (Some seq_init) cm).1 with
+  | Some _ => True
+  | None => False
+  end.
+
+Fixpoint well_defined_stmts ss cm seq_init : Prop :=
+  match ss with
+  | Qnil => True
+  | Qcons s st => match (expandBranch_funs st (Some (Qnil ProdVarOrder.T)) (expandBranch_fun s (Some (Qnil ProdVarOrder.T)) cm).1) with
+                  | Some _ => True
+                  | None => False
+                  end
+  end.*)
+
+(* old version
+
+Definition expandBranch_declaration_stmts_match (ss : HiFP.hfstmt_seq) : Prop :=
+  forall ce cm thfstmt envce,
+  (*well_defined_stmts ss cm (Qnil ProdVarOrder.T) ->*)
+  fst (expandBranch_funs ss (Some (Qnil ProdVarOrder.T)) cm) = Some thfstmt ->
+  CEP.Equal (expandBranch_declarations ce ss envce) (expandBranch_declarations ce thfstmt envce).
+
+Lemma ExpandWhens_declarations_correct :
+  forall (ss : HiFP.hfstmt_seq),
+  expandBranch_declaration_stmts_match ss
+with ExpandBranch_declaration_when :
+  forall s,
+  match s with
+  | Swhen c s1 s2 => expandBranch_declaration_stmts_match s1 /\ expandBranch_declaration_stmts_match s2
+  | _ => True
+  end.
+Proof.
+  clear ExpandWhens_declarations_correct.
+  induction ss.
+  - rewrite /expandBranch_declaration_stmts_match.
+    simpl.
+    move => ce cm thfstmt envce Hseq.
+    inversion Hseq.
+    rewrite /expandBranch_declarations //.
+  - rewrite /expandBranch_declaration_stmts_match.
+    move => ce cm thfstmt envce Hseq.
+    rewrite /expandBranch_declaration_stmts_match in IHss.
+    simpl in Hseq.
+    simpl.
+    move : Hseq.
+    case Hh : h => [|v t|||||||c ts fs]; try done.
+      - simpl.
+      apply IHss.
+      (*rewrite Hh in H.
+      simpl in H.
+      move : H => [_ H].
+      apply H. 
+      done.*)
+      - intro.
+      simpl in Hseq.
+      case Hcons : (expandBranch_funs ss (Some (Qnil ProdVarOrder.T)) (CEP.add v D_undefined cm)).1 => [tss|].
+      specialize cons_expandBranch_declarations with (ss := ss) (seq_init := (Qcons (Swire (var:=ProdVarOrder.T) v t) (Qnil ProdVarOrder.T))) (cm_result := (CEP.add v D_undefined cm)) 
+        (seq_result := tss).
+      move => Hcons'.
+      generalize Hcons.
+      apply Hcons' in Hcons.
+      clear Hcons'.
+      move => Hcons'.
+      rewrite Hcons in Hseq. 
+      inversion Hseq.
+      rewrite cat_expandBranch_delarations.
+
+      specialize IHss with (ce := (match CEP.find v ce with
+        | Some _ => CEP.remove v ce
+        | None => CEP.add v (HiFP.aggr_typ t, Wire) ce
+        end)) (cm := (CEP.add v D_undefined cm)) (envce := envce) (thfstmt := tss).
+
+      simpl.
+      rewrite IHss //.
+      admit.
+      (* (expandBranch_funs ss
+           (Some (Qnil ProdVarOrder.T))
+           (CEP.add v D_undefined cm)).1 =
+        None *)
+
+      admit.
+      admit.
+      admit.
+      admit.
+      admit.
+      admit.
+      (* when *)
+      intro.
+      specialize ExpandBranch_declaration_when with (s := (Swhen c ts fs)).
+      simpl in ExpandBranch_declaration_when.
+      move : ExpandBranch_declaration_when => [Ht Hf].
+      (*case Hcons : (expandBranch_funs ss (Some (Qnil ProdVarOrder.T)) (CEP.add v D_undefined cm)).1 => [tss|].
+
+      simpl in Hseq.
+      simpl.
+
+      - (* wire,register,mem,node,inst *)
+      1,2,3,4,5: intros.
+      1,2,3,4,5: rewrite cons_expandBranch_declarations.
+      1,2,3,4,5: rewrite cat_expandBranch_delarations.
+      1,2,3,4,5: simpl.
+      specialize IHss with (ce_other_modules := ce_other_modules) (cm_init := (init_ref s f cm_init)) (init_decl_map := (CEP.add s (HiFP.aggr_typ f, Wire) init_decl_map)) (ce := ce).
+      exact IHss.
+      specialize IHss with (ce_other_modules := ce_other_modules) (cm_init := (init_register s (type h0) cm_init)) (init_decl_map := (CEP.add s (HiFP.reg_typ h0, Register) init_decl_map)) (ce := ce).
+      exact IHss.
+      specialize IHss with (ce_other_modules := ce_other_modules) (cm_init := cm_init) (init_decl_map := (CEP.add s (HiFP.mem_typ h0, Memory) init_decl_map)) (ce := ce).
+      exact IHss.
+      specialize IHss with (ce_other_modules := ce_other_modules) (cm_init := cm_init) (init_decl_map := (CEP.add s ((CEP.vtyp s0 ce).1, Instanceof) init_decl_map)) (ce := ce).
+      exact IHss.
+      specialize IHss with (ce_other_modules := ce_other_modules) (cm_init := cm_init) (init_decl_map := (CEP.add s (HiFP.aggr_typ (HiFP.type_of_hfexpr h0 ce), Node) init_decl_map)) (ce := ce).
+      exact IHss.
+      - (* cnct *)
+      intros.
+      case h0 => [r|||]; try done.
+      - (* invalid *)
+      intros.
+      case h0 => [r|||]; try done.
+      - (* when *)
+      specialize ExpandWhens_declarations_correct_Swhen with (s := (Swhen c ts fs)).
+      simpl in ExpandWhens_declarations_correct_Swhen.
+      move : ExpandWhens_declarations_correct_Swhen => [Ht Hf].
+
+      case Hcombine : (combine_branches c
+        (expandBranch_fun ts ce_other_modules
+          (Qnil ProdVarOrder.T) cm_init)
+        (expandBranch_fun fs ce_other_modules
+          (Qnil ProdVarOrder.T) cm_init)) => [new_hseq new_cm].
+      rewrite cons_expandBranch_declarations.
+      rewrite cat_expandBranch_delarations.
+      have ->: new_hseq = fst (combine_branches c
+        (expandBranch_fun ts ce_other_modules
+          (Qnil ProdVarOrder.T) cm_init)
+        (expandBranch_fun fs ce_other_modules
+          (Qnil ProdVarOrder.T) cm_init)) by rewrite Hcombine.
+      rewrite /combine_branches.
+      simpl.
+      clear Hcombine.
+      rewrite /ExpandBranch_declarations_is_correct in Ht.
+      rewrite /ExpandBranch_declarations_is_correct in Hf. 
+      assert (Hcombine : (expandBranch_declarations
+        (expandBranch_declarations init_decl_map ts ce) fs ce) = (expandBranch_declarations init_decl_map
+        (Qcat
+           (expandBranch_fun ts ce_other_modules
+              (Qnil ProdVarOrder.T) cm_init).1
+           (expandBranch_fun fs ce_other_modules
+              (Qnil ProdVarOrder.T) cm_init).1) ce)).
+      admit.
+      rewrite -Hcombine.
+      specialize IHss with (ce_other_modules := ce_other_modules) (cm_init := new_cm) (init_decl_map := (expandBranch_declarations
+      (expandBranch_declarations init_decl_map ts ce) fs ce)) (ce := ce).
+      exact IHss.
+  
+  (* prove ExpandWhens_declarations_correct_Swhen *)
+  clear ExpandWhens_declarations_correct_Swhen.
+  intro.
+  destruct s; try done.
+  Admitted.
+
+  (* CEP.Lemmas.add_same:
+  forall [elt : Type] [x : PVM.key] [e : elt] [m : PVM.t elt],
+  PVM.find x m = Some e -> PVM.Equal (PVM.add x e m) m 
+
+  CEP.Lemmas.add_m:
+  forall [elt : Type] [x y : PVM.SE.t],
+  PVM.SE.eq x y ->
+  forall x0 y0 : elt,
+  x0 = y0 ->
+  forall x1 y1 : PVM.t elt,
+  PVM.Equal x1 y1 -> PVM.Equal (PVM.add x x0 x1) (PVM.add y y0 y1)*)
+  *)
+  Admitted.*)
+
+Lemma expandBranch_declaration_skip_match :
+  forall ce seq_init cm thfstmt envce,
+  fst (expandBranch_fun (HiFP.sskip) (Some seq_init) cm) = Some thfstmt ->
+  expandBranch_declaration_stmt (HiFP.sskip) seq_init ce (expandBranch_declarations ce thfstmt envce).
+Proof.
+  intros.
+  apply ExpandBranch_declaration_skip.
+Qed.
+  
+Lemma expandBranch_declaration_wire_match :
+  forall v t ce seq_init envce thfstmt cm,
+  (*~~ CEP.mem v ce ->*)
+  fst (expandBranch_fun (Swire v t) (Some seq_init) cm) = Some thfstmt ->
+  expandBranch_declaration_stmt (Swire v t) seq_init ce (expandBranch_declarations ce thfstmt envce).
+Proof.
+  move => v t ce seq_init envce thfstmt cm H0.
+  apply ExpandBranch_declaration_wire with (envce := envce).
+  simpl in H0. 
+  case Hin : (Qin (Swire v t) seq_init).
+  - rewrite Hin in H0. 
+    discriminate.
+  - rewrite Hin in H0. 
+    inversion H0. 
+    simpl.
+    apply HiFP.PCELemmas.Equal_refl.
+  Qed.
+
+Lemma expandBranch_declaration_reg_match :
+  forall v r ce seq_init envce thfstmt cm,
+  fst (expandBranch_fun (Sreg v r) (Some seq_init) cm) = Some thfstmt ->
+  expandBranch_declaration_stmt (Sreg v r) seq_init ce (expandBranch_declarations ce thfstmt envce).
+Proof.
+  move => v r ce seq_init envce thfstmt cm H0.
+  apply ExpandBranch_declaration_reg with (envce := envce).
+  simpl in H0. 
+  case Hin : (Qin (Sreg v r) seq_init).
+  - rewrite Hin in H0. 
+    discriminate.
+  - rewrite Hin in H0. 
+    inversion H0. 
+    simpl.
+    apply HiFP.PCELemmas.Equal_refl.
+  Qed.
+
+Lemma expandBranch_declaration_mem_match :
+  forall v t ce seq_init envce thfstmt cm,
+  fst (expandBranch_fun (Smem v t) (Some seq_init) cm) = Some thfstmt ->
+  expandBranch_declaration_stmt (Smem v t) seq_init ce (expandBranch_declarations ce thfstmt envce).
+Proof.
+  move => v t ce seq_init envce thfstmt cm H0.
+  apply ExpandBranch_declaration_mem with (envce := envce).
+  simpl in H0. 
+  case Hin : (Qin (Smem v t) seq_init).
+  - rewrite Hin in H0. 
+    discriminate.
+  - rewrite Hin in H0. 
+    inversion H0. 
+    simpl.
+    apply HiFP.PCELemmas.Equal_refl.
+  Qed.
+  
+Lemma expandBranch_declaration_node_match :
+  forall v t ce seq_init envce thfstmt cm,
+  fst (expandBranch_fun (Snode v t) (Some seq_init) cm) = Some thfstmt ->
+  expandBranch_declaration_stmt (Snode v t) seq_init ce (expandBranch_declarations ce thfstmt envce).
+Proof.
+  move => v t ce seq_init envce thfstmt cm H0.
+  apply ExpandBranch_declaration_node with (envce := envce).
+  simpl in H0. 
+  case Hin : (Qin (Snode v t) seq_init).
+  - rewrite Hin in H0. 
+    discriminate.
+  - rewrite Hin in H0. 
+    inversion H0. 
+    simpl.
+    apply HiFP.PCELemmas.Equal_refl.
+  Qed.
+
+Lemma expandBranch_declaration_inst_match :
+  forall v t ce seq_init envce thfstmt cm,
+  fst (expandBranch_fun (Sinst v t) (Some seq_init) cm) = Some thfstmt ->
+  expandBranch_declaration_stmt (Sinst v t) seq_init ce (expandBranch_declarations ce thfstmt envce).
+Proof.
+  move => v t ce seq_init envce thfstmt cm H0.
+  apply ExpandBranch_declaration_inst with (envce := envce).
+  simpl in H0. 
+  case Hin : (Qin (Sinst v t) seq_init).
+  - rewrite Hin in H0. 
+    discriminate.
+  - rewrite Hin in H0. 
+    inversion H0. 
+    simpl.
+    apply HiFP.PCELemmas.Equal_refl.
+  Qed.
+
+Lemma expandBranch_declaration_invalid_match :
+  forall v ce seq_init envce thfstmt cm,
+  fst (expandBranch_fun (Sinvalid v) (Some seq_init) cm) = Some thfstmt ->
+  expandBranch_declaration_stmt (Sinvalid v) seq_init ce (expandBranch_declarations ce thfstmt envce).
+Proof.
+  move => v ce seq_init envce thfstmt cm H0.
+  apply ExpandBranch_declaration_invalid with (envce := envce).
+  simpl in H0.
+  move : H0. 
+  case : v.
+  1,2,3,4: intros.
+  1,2,3,4: simpl.
+  1,2,3,4: simpl in H0.
+  1,2,3,4: inversion H0.
+  1,2,3,4: apply HiFP.PCELemmas.Equal_refl.
+  Qed.
+  
+Lemma expandBranch_declaration_fcnct_match :
+  forall v e ce seq_init envce thfstmt cm,
+  fst (expandBranch_fun (Sfcnct v e) (Some seq_init) cm) = Some thfstmt ->
+  expandBranch_declaration_stmt (Sfcnct v e) seq_init ce (expandBranch_declarations ce thfstmt envce).
+Proof.
+  move => v e ce seq_init envce thfstmt cm H0.
+  apply ExpandBranch_declaration_fcnct with (envce := envce).
+  simpl in H0.
+  move : H0. 
+  case : v.
+  1,2,3,4: intros.
+  1,2,3,4: simpl.
+  1,2,3,4: simpl in H0.
+  1,2,3,4: inversion H0.
+  1,2,3,4: apply HiFP.PCELemmas.Equal_refl.
+  Qed.
+
+Lemma expandBranch_declaration_when_match :
+  forall c s1 s2 ce seq_init envce thfstmt cm seq_init',
+  fst (expandBranch_funs s1 (Some seq_init) cm) = Some seq_init' ->
+  fst (expandBranch_fun (Swhen c s1 s2) (Some seq_init) cm) = Some thfstmt ->
+  expandBranch_declaration_stmts s1 seq_init ce (expandBranch_declarations ce seq_init' envce) ->
+  expandBranch_declaration_stmts s2 seq_init' ce (expandBranch_declarations ce thfstmt envce) ->
+  expandBranch_declaration_stmt (Swhen c s1 s2) seq_init ce (expandBranch_declarations ce thfstmt envce).
+Proof.
+  intros.
+  apply ExpandBranch_declaration_when with (seq_init' := seq_init') (ce' := (expandBranch_declarations ce seq_init' envce)); try by done.
+Qed.
+
+Lemma expandBranch_declaration_match (s : HiFP.hfstmt) :
+  forall ce envce thfstmt seq_init cm,
+  fst (expandBranch_fun s (Some seq_init) cm) = Some thfstmt ->
+  expandBranch_declaration_stmt s seq_init ce (expandBranch_declarations ce thfstmt envce)
+with expandBranch_declarations_match (ss : HiFP.hfstmt_seq) :
+  forall ce envce thfstmt seq_init cm,
+  fst (expandBranch_funs ss (Some seq_init) cm) = Some thfstmt ->
+  expandBranch_declaration_stmts ss seq_init ce (expandBranch_declarations ce thfstmt envce).
+Proof.
+  clear expandBranch_declaration_match.
+  case Hs : s => [|v t|||||||c s1 s2]; try done.
+  - move => ce envce thfstmt seq_init cm.
+    apply expandBranch_declaration_skip_match.
+  - move => ce envce thfstmt seq_init cm.
+    apply expandBranch_declaration_wire_match.
+  - move => ce envce thfstmt seq_init cm.
+    apply expandBranch_declaration_reg_match.
+  - move => ce envce thfstmt seq_init cm.
+    apply expandBranch_declaration_mem_match.
+  - move => ce envce thfstmt seq_init cm.
+    apply expandBranch_declaration_inst_match.
+  - move => ce envce thfstmt seq_init cm.
+    apply expandBranch_declaration_node_match.
+  - move => ce envce thfstmt seq_init cm.
+    apply expandBranch_declaration_fcnct_match.
+  - move => ce envce thfstmt seq_init cm.
+    apply expandBranch_declaration_invalid_match.
+  - intros.
+    case Hf : (fst (expandBranch_funs s1 (Some seq_init) cm)) => [seq_init'|].
+    apply expandBranch_declaration_when_match with (cm := cm) (seq_init' := seq_init'); try by done.
+    apply expandBranch_declarations_match with (cm := cm); try by done.
+    simpl in H.
+    rewrite Hf in H. 
+    apply expandBranch_declarations_match with (cm := cm); try by done.
+    admit. (* (expandBranch_funs s1 (Some seq_init) cm).1 = None *)
+  clear expandBranch_declarations_match.
+  induction ss.
+  - simpl.
+    intros.
+    inversion H. 
+    simpl.
+    apply ExpandBranch_declarations_nil.
+    - intros.
+    case Hf : ((expandBranch_fun h (Some seq_init) cm).1) => [seq_init'|].
+    apply ExpandBranch_declarations_con with (s := h) (ss := ss) (seq_init := seq_init) 
+    (seq_init' := seq_init') (ce := ce) (ce' := (expandBranch_declarations ce seq_init' envce)); try by done.
+    apply expandBranch_declaration_match with (cm := cm); try by done.
+    simpl in H.
+    apply IHss with (cm:= (snd (expandBranch_fun h (Some seq_init) cm))); try by done.
+    rewrite -Hf //.
+Admitted.
+
+
+
+(* Proof of connections *)
+Inductive expr_tree : Type :=
+  (*| T_undeclared (* in this execution path, the component is not declared *) *)
+  | T_undefined (* the component is erroneously not connected *)
+  | T_invalidated (* the component is not connected but the programmer has
+                    indicated with an "is invalid" statement that this is ok *)
+  | T_fexpr : HiFP.hfexpr -> expr_tree
+  | T_choice : HiFP.hfexpr (* condition *) ->
+              expr_tree (* choice if condition is true *) ->
+              expr_tree (* choice if condition is false *) -> expr_tree
+  .
+  
+Definition helper_tree (c : HiFP.hfexpr) (true_tree : option expr_tree) (false_tree : option expr_tree) : option expr_tree := 
+  match true_tree, false_tree with
+  (*| Some T_undeclared, _ => false_tree
+  | _, Some T_undeclared => true_tree*)
+  | None, None => None
+  | Some T_invalidated, _ => false_tree
+  | _, Some T_invalidated => true_tree
+  | Some T_undefined, _ => false_tree (* 任何branch有undefined都是错误 *)
+  | _, Some T_undefined => true_tree (* 任何branch有undefined都是错误 *)
+  | Some tree1, Some tree2 => Some (T_choice c tree1 tree2)
+  | _, _ => true_tree
+  end.
+
+Fixpoint expandBranch_connection_tree (s : HiFP.hfstmt) (expr_tree_map : CEP.t expr_tree) : CEP.t expr_tree :=
+  match s with
+  | Swire v _
+  | Smem v _
+  | Sinst v _ => CEP.add v T_undefined expr_tree_map 
+  | Sreg v r => CEP.add v (T_fexpr (Eref (Eid v))) expr_tree_map
+  | Sfcnct (Eid r) e => CEP.add r (T_fexpr e) expr_tree_map
+  | Sinvalid (Eid r) => CEP.add r T_invalidated expr_tree_map
+  | Swhen c s1 s2 => let true_child := expandBranch_connection_trees s1 expr_tree_map in
+                     let false_child := expandBranch_connection_trees s2 expr_tree_map in
+                     CEP.map2 (helper_tree c) true_child false_child
+  | _ => expr_tree_map
+  end
+with expandBranch_connection_trees (ss : HiFP.hfstmt_seq) (expr_tree_map : CEP.t expr_tree) : CEP.t expr_tree :=
+  match ss with
+  | Qnil => expr_tree_map
+  | Qcons s st => let new_expr_tree_map := expandBranch_connection_tree s expr_tree_map in
+                  expandBranch_connection_trees st new_expr_tree_map
+  end.
+
+(*Definition ce0 :CEP.env:= CEP.empty (cmpnt_init_typs ProdVarOrder.T * fcomponent).
+Definition agt := HiFP.aggr_typ (Gtyp (Fuint 1)).
+
+Definition p1 : pvar := (N.of_nat 1, N0).
+Definition p2 : pvar := (N.of_nat 2, N0).
+Definition ec0 := (HiFP.econst (Fuint 1) [::false]).
+Definition ec1 := (HiFP.econst (Fuint 2) [::false;false]).
+Definition ec2 := (HiFP.econst (Fuint 2) [::false;true]).
+Definition ec3 := (HiFP.econst (Fuint 2) [::true;true]).
+Definition ty0 := Gtyp (Fuint 2).
+Definition es1 := Swire p1 ty0.
+Definition esinvalid := Sinvalid (Eid p1).
+Definition est := Sfcnct (Eid p1) ec2.
+Definition esf := Sfcnct (Eid p1) ec3.
+Definition esw := Swhen ec0 (Qcons est (Qnil ProdVarOrder.T)) ((Qnil ProdVarOrder.T)).
+Definition ess := Qcons es1 (Qcons esf (Qcons esw (Qnil ProdVarOrder.T))).
+
+Definition temp_tree_map := expandBranch_connection_tree ess (CEP.empty expr_tree).
+Definition a_tree := CEP.find p1 temp_tree_map.
+Compute (a_tree).*)
+
+Fixpoint connection_tree2expr (tree: expr_tree) : option def_expr :=
+  match tree with
+  (*| T_undeclared => None*)
+  | T_undefined => Some D_undefined
+  | T_invalidated => Some D_invalidated
+  | T_fexpr e => Some (D_fexpr e)
+  | T_choice cond true_tree false_tree => let true_expr := connection_tree2expr true_tree in
+                                          let false_expr := connection_tree2expr false_tree in
+                                          match true_expr, false_expr with
+                                          | Some (D_fexpr te), Some (D_fexpr fe) => (*if te == fe then Some (D_fexpr te)
+                                                        else*) Some (D_fexpr (Emux cond te fe))
+                                          | Some D_invalidated, Some (D_fexpr fe) => false_expr
+                                          | Some (D_fexpr fe), Some D_invalidated => true_expr
+                                          | _, _ => true_expr
+                                          end
+   end.
+
+Definition texpr_match_ttree cm tm : Prop :=
+  forall v texpr1 ttree1,
+  CEP.find v cm = texpr1 ->
+  CEP.find v tm = Some ttree1 ->
+  texpr1 = connection_tree2expr ttree1.
+
+Inductive expandBranch_connection_stmt : HiFP.hfstmt -> CEP.t def_expr -> CEP.t def_expr -> CEP.t expr_tree -> CEP.t expr_tree -> Prop :=
+  | ExpandBranch_connection_skip cm cm' tm tm':
+      expandBranch_connection_stmt (HiFP.sskip) cm cm' tm tm'
+  (* old version
+  | ExpandBranch_connection_wire v t cm cm' tm tm':
+      forall texpr ttree,
+      CEP.find v cm' = texpr -> (* D_undefined *)
+      CEP.find v tm' = Some ttree -> 
+      texpr = connection_tree2expr ttree ->
+      expandBranch_connection_stmt (Swire v t) cm cm' tm tm'
+  | ExpandBranch_connection_reg v r cm cm' tm tm' :
+      forall texpr ttree,
+      CEP.find v cm' = texpr -> (* D_expr (Eid r) *)
+      CEP.find v tm' = Some ttree -> 
+      texpr = connection_tree2expr ttree ->
+      expandBranch_connection_stmt (Sreg v r) cm cm' tm tm'
+  | ExpandBranch_connection_inst v1 v2 cm cm' tm tm':
+      forall texpr ttree,
+      CEP.find v1 cm' = texpr -> (* D_undefined *)
+      CEP.find v1 tm' = Some ttree -> 
+      texpr = connection_tree2expr ttree ->
+      expandBranch_connection_stmt (Sinst v1 v2) cm cm' tm tm'
+  | ExpandBranch_connection_node v e cm tm:
+      expandBranch_connection_stmt (Snode v e) cm cm tm tm
+  | ExpandBranch_connection_mem v m cm cm' tm tm' :
+      forall texpr ttree,
+      CEP.find v cm' = texpr -> (* D_undefined *)
+      CEP.find v tm' = Some ttree -> 
+      texpr = connection_tree2expr ttree ->
+      expandBranch_connection_stmt (Smem v m) cm cm' tm tm'
+  | ExpandBranch_connection_invalid v cm cm' tm tm':
+      forall texpr ttree,
+      CEP.find v cm' = texpr -> (* D_invalid *)
+      CEP.find v tm' = Some ttree -> 
+      texpr = connection_tree2expr ttree ->
+      expandBranch_connection_stmt (Sinvalid (Eid v)) cm cm' tm tm'
+  | ExpandBranch_connection_fcnct v e cm cm' tm tm':
+      forall texpr ttree,
+      CEP.find v cm' = texpr -> (* D_expr *)
+      CEP.find v tm' = Some ttree -> 
+      texpr = connection_tree2expr ttree ->
+      expandBranch_connection_stmt (Sfcnct (Eid v) e) cm cm' tm tm'
+  | ExpandBranch_connection_when c s1 s2 cm cm' cm'' cm0 tm tm' tm' tm0 :
+      expandBranch_connection_stmts s1 cm cm' tm tm' ->
+      expandBranch_connection_stmts s2 cm cm'' tm tm'' ->
+      (forall v texpr1 texpr2 ttree1 ttree2 ttree',
+      CEP.mem v cm0 /\ CEP.mem v tm0 ->
+      CEP.find v cm' = texpr1 ->
+      CEP.find v cm'' = texpr2 ->
+      CEP.find v tm' = Some ttree1 ->
+      CEP.find v tm'' = Some ttree2 ->
+      helper_tree c (Some ttree1) (Some ttree2) = Some ttree' ->
+      helper_tf c texpr1 texpr2 = connection_tree2expr ttree'
+      ) ->
+      expandBranch_connection_stmt (Swhen c s1 s2) cm cm0 tm tm0
+  *)
+  | ExpandBranch_connection_wire v t cm cm' tm tm':
+      texpr_match_ttree cm tm ->
+      texpr_match_ttree cm' tm' ->
+      expandBranch_connection_stmt (Swire v t) cm cm' tm tm'
+  | ExpandBranch_connection_reg v r cm cm' tm tm' :
+      texpr_match_ttree cm tm ->
+      texpr_match_ttree cm' tm' ->
+      expandBranch_connection_stmt (Sreg v r) cm cm' tm tm'
+  | ExpandBranch_connection_inst v1 v2 cm cm' tm tm':
+      texpr_match_ttree cm tm ->
+      texpr_match_ttree cm' tm' ->
+      expandBranch_connection_stmt (Sinst v1 v2) cm cm' tm tm'
+  | ExpandBranch_connection_node v e cm cm' tm tm':
+      texpr_match_ttree cm tm ->
+      texpr_match_ttree cm' tm' ->
+      expandBranch_connection_stmt (Snode v e) cm cm tm tm
+  | ExpandBranch_connection_mem v m cm cm' tm tm' :
+      texpr_match_ttree cm tm ->
+      texpr_match_ttree cm' tm' ->
+      expandBranch_connection_stmt (Smem v m) cm cm' tm tm'
+  | ExpandBranch_connection_invalid v cm cm' tm tm':
+      texpr_match_ttree cm tm ->
+      texpr_match_ttree cm' tm' ->
+      expandBranch_connection_stmt (Sinvalid (Eid v)) cm cm' tm tm'
+  | ExpandBranch_connection_fcnct v e cm cm' tm tm':
+      texpr_match_ttree cm tm ->
+      texpr_match_ttree cm' tm' ->
+      expandBranch_connection_stmt (Sfcnct (Eid v) e) cm cm' tm tm'
+  | ExpandBranch_connection_when c s1 s2 cm cm0 tm tm0 :
+      texpr_match_ttree cm tm ->
+      texpr_match_ttree cm0 tm0 ->
+      expandBranch_connection_stmt (Swhen c s1 s2) cm cm0 tm tm0
+
+with expandBranch_connection_stmts : HiFP.hfstmt_seq -> CEP.t def_expr -> CEP.t def_expr -> CEP.t expr_tree -> CEP.t expr_tree -> Prop :=
+  | ExpandBranch_connections_nil cm tm :
+      expandBranch_connection_stmts HiFP.qnil cm cm tm tm
+  | ExpandBranch_connections_con s ss cm cm' cm'' tm tm' tm'':
+      expandBranch_connection_stmt s cm cm' tm tm' ->
+      expandBranch_connection_stmts ss cm' cm'' tm' tm'' ->
+      expandBranch_connection_stmts (Qcons s ss) cm cm'' tm tm''.
+
+(* old version
+  for every statement case only look at the corresponding varaiable, hard to use to handle statement sequence.
+Lemma expandBranch_connection_wire_match :
+  forall v ty cm tm seq_result texpr ttree,
+  CEP.find v (snd (expandBranch_fun (Swire v ty) seq_result cm)) = texpr -> 
+  CEP.find v (expandBranch_connection_tree (Swire v ty) tm) = Some ttree -> 
+  expandBranch_connection_stmt (Swire v ty) cm (snd (expandBranch_fun (Swire v ty) seq_result cm)) tm (expandBranch_connection_tree (Swire v ty) tm).
+Proof.
+  intros.
+  apply ExpandBranch_connection_wire with (texpr := texpr) (ttree := ttree); try done.
+  rewrite /expandBranch_fun in H. 
+  simpl in H. 
+  assert (Hfindadd : CEP.find v (CEP.add v D_undefined cm) = Some D_undefined).
+  apply HiFP.PCELemmas.add_eq_o.
+  apply CEP.SE.eq_refl.
+  rewrite Hfindadd in H.
+  clear Hfindadd.
+  rewrite -H.
+  rewrite /expandBranch_connection_tree in H0.
+  assert (Hfindadd : CEP.find v (CEP.add v T_undefined tm) = Some T_undefined).
+  apply HiFP.PCELemmas.add_eq_o.
+  apply CEP.SE.eq_refl.
+  rewrite Hfindadd in H0.
+  clear Hfindadd.
+  inversion H0.
+  rewrite /connection_tree2expr //.
+Qed.
+*)
+
+(* new lemma should prove that after dealing with any single statement, for every element, its texpr and ttree match property should hold. *)
+Lemma expandBranch_connection_wire_match :
+  forall v ty cm cm' tm tm' seq_result,
+  texpr_match_ttree cm tm ->
+  cm' = snd (expandBranch_fun (Swire v ty) seq_result cm) -> 
+  tm' = expandBranch_connection_tree (Swire v ty) tm -> 
+  expandBranch_connection_stmt (Swire v ty) cm cm' tm tm'.
+Proof.
+  move => v ty cm cm' tm tm' seq_result Hpre Hcm' Htm'.
+  apply ExpandBranch_connection_wire; try by done.
+  simpl in Hcm'.
+  simpl in Htm'.
+  rewrite /texpr_match_ttree in Hpre.
+  rewrite /texpr_match_ttree.
+  move => v1 texpr1 ttree1.
+  (* discuss on whether v1 equals to v? *)
+Admitted.
+
+(* old version on all the other single statement case
+Lemma expandBranch_connection_reg_match :
+  forall v r cm tm seq_result texpr ttree,
+  CEP.find v (snd (expandBranch_fun (Sreg v r) seq_result cm)) = texpr -> 
+  CEP.find v (expandBranch_connection_tree (Sreg v r) tm) = Some ttree -> 
+  expandBranch_connection_stmt (Sreg v r) cm (snd (expandBranch_fun (Sreg v r) seq_result cm)) tm (expandBranch_connection_tree (Sreg v r) tm).
+Proof.
+  intros.
+  apply ExpandBranch_connection_reg with (texpr := texpr) (ttree := ttree); try done.
+  rewrite /expandBranch_fun in H. 
+  simpl in H. 
+  assert (Hfindadd : CEP.find v (CEP.add v (D_fexpr (Eref (Eid (var:=ProdVarOrder.T) v))) cm) = Some (D_fexpr (Eref (Eid (var:=ProdVarOrder.T) v)))).
+  apply HiFP.PCELemmas.add_eq_o.
+  apply CEP.SE.eq_refl.
+  rewrite Hfindadd in H.
+  clear Hfindadd.
+  rewrite -H.
+  rewrite /expandBranch_connection_tree in H0.
+  assert (Hfindadd : CEP.find v (CEP.add v (T_fexpr (Eref (Eid (var:=ProdVarOrder.T) v))) tm) = Some (T_fexpr (Eref (Eid (var:=ProdVarOrder.T) v)))).
+  apply HiFP.PCELemmas.add_eq_o.
+  apply CEP.SE.eq_refl.
+  rewrite Hfindadd in H0.
+  clear Hfindadd.
+  inversion H0.
+  rewrite /connection_tree2expr //.
+Qed.
+
+Lemma expandBranch_connection_inst_match :
+  forall v1 v2 cm tm seq_result texpr ttree,
+  CEP.find v1 (snd (expandBranch_fun (Sinst v1 v2) seq_result cm)) = texpr -> 
+  CEP.find v1 (expandBranch_connection_tree (Sinst v1 v2) tm) = Some ttree -> 
+  expandBranch_connection_stmt (Sinst v1 v2) cm (snd (expandBranch_fun (Sinst v1 v2) seq_result cm)) tm (expandBranch_connection_tree (Sinst v1 v2) tm).
+Proof.
+  intros.
+  apply ExpandBranch_connection_inst with (texpr := texpr) (ttree := ttree); try done.
+  rewrite /expandBranch_fun in H. 
+  simpl in H. 
+  assert (Hfindadd : CEP.find v1 (CEP.add v1 (D_undefined) cm) = Some (D_undefined)).
+  apply HiFP.PCELemmas.add_eq_o.
+  apply CEP.SE.eq_refl.
+  rewrite Hfindadd in H.
+  clear Hfindadd.
+  rewrite -H.
+  rewrite /expandBranch_connection_tree in H0.
+  assert (Hfindadd : CEP.find v1 (CEP.add v1 (T_undefined) tm) = Some (T_undefined)).
+  apply HiFP.PCELemmas.add_eq_o.
+  apply CEP.SE.eq_refl.
+  rewrite Hfindadd in H0.
+  clear Hfindadd.
+  inversion H0.
+  rewrite /connection_tree2expr //.
+Qed.
+
+Lemma expandBranch_connection_snode_match :
+  forall v e cm tm seq_result,
+  expandBranch_connection_stmt (Snode v e) cm (snd (expandBranch_fun (Snode v e) seq_result cm)) tm (expandBranch_connection_tree (Snode v e) tm).
+Proof.
+  intros.
+  apply ExpandBranch_connection_node.
+Qed.
+
+Lemma expandBranch_connection_mem_match :
+  forall v m cm tm seq_result texpr ttree,
+  CEP.find v (snd (expandBranch_fun (Smem v m) seq_result cm)) = texpr -> 
+  CEP.find v (expandBranch_connection_tree (Smem v m) tm) = Some ttree -> 
+  expandBranch_connection_stmt (Smem v m) cm (snd (expandBranch_fun (Smem v m) seq_result cm)) tm (expandBranch_connection_tree (Smem v m) tm).
+Proof.
+  intros.
+  apply ExpandBranch_connection_mem with (texpr := texpr) (ttree := ttree); try done.
+  rewrite /expandBranch_fun in H. 
+  simpl in H. 
+  assert (Hfindadd : CEP.find v (CEP.add v D_undefined cm) = Some D_undefined).
+  apply HiFP.PCELemmas.add_eq_o.
+  apply CEP.SE.eq_refl.
+  rewrite Hfindadd in H.
+  clear Hfindadd.
+  rewrite -H.
+  rewrite /expandBranch_connection_tree in H0.
+  assert (Hfindadd : CEP.find v (CEP.add v T_undefined tm) = Some T_undefined).
+  apply HiFP.PCELemmas.add_eq_o.
+  apply CEP.SE.eq_refl.
+  rewrite Hfindadd in H0.
+  clear Hfindadd.
+  inversion H0.
+  rewrite /connection_tree2expr //.
+Qed.
+
+Lemma expandBranch_connection_invalid_match :
+  forall v cm tm seq_result texpr ttree,
+  CEP.find v (snd (expandBranch_fun (Sinvalid (Eid v)) seq_result cm)) = texpr -> 
+  CEP.find v (expandBranch_connection_tree (Sinvalid (Eid v)) tm) = Some ttree -> 
+  expandBranch_connection_stmt (Sinvalid (Eid v)) cm (snd (expandBranch_fun (Sinvalid (Eid v)) seq_result cm)) tm (expandBranch_connection_tree (Sinvalid (Eid v)) tm).
+Proof.
+  intros.
+  apply ExpandBranch_connection_invalid with (texpr := texpr) (ttree := ttree); try done.
+  rewrite /expandBranch_fun in H. 
+  simpl in H. 
+  assert (Hfindadd : CEP.find v (CEP.add v D_invalidated cm) = Some D_invalidated).
+  apply HiFP.PCELemmas.add_eq_o.
+  apply CEP.SE.eq_refl.
+  rewrite Hfindadd in H.
+  clear Hfindadd.
+  rewrite -H.
+  rewrite /expandBranch_connection_tree in H0.
+  assert (Hfindadd : CEP.find v (CEP.add v T_invalidated tm) = Some T_invalidated).
+  apply HiFP.PCELemmas.add_eq_o.
+  apply CEP.SE.eq_refl.
+  rewrite Hfindadd in H0.
+  clear Hfindadd.
+  inversion H0.
+  rewrite /connection_tree2expr //.
+Qed.
+
+Lemma expandBranch_connection_fcnct_match :
+  forall v e cm tm seq_result texpr ttree,
+  CEP.find v (snd (expandBranch_fun (Sfcnct (Eid v) e) seq_result cm)) = texpr -> 
+  CEP.find v (expandBranch_connection_tree (Sfcnct (Eid v) e) tm) = Some ttree -> 
+  expandBranch_connection_stmt (Sfcnct (Eid v) e) cm (snd (expandBranch_fun (Sfcnct (Eid v) e) seq_result cm)) tm (expandBranch_connection_tree (Sfcnct (Eid v) e) tm).
+Proof.
+  intros.
+  apply ExpandBranch_connection_fcnct with (texpr := texpr) (ttree := ttree); try done.
+  rewrite /expandBranch_fun in H. 
+  simpl in H. 
+  assert (Hfindadd : CEP.find v (CEP.add v (D_fexpr e) cm) = Some (D_fexpr e)).
+  apply HiFP.PCELemmas.add_eq_o.
+  apply CEP.SE.eq_refl.
+  rewrite Hfindadd in H.
+  clear Hfindadd.
+  rewrite -H.
+  rewrite /expandBranch_connection_tree in H0.
+  assert (Hfindadd : CEP.find v (CEP.add v (T_fexpr e) tm) = Some (T_fexpr e)).
+  apply HiFP.PCELemmas.add_eq_o.
+  apply CEP.SE.eq_refl.
+  rewrite Hfindadd in H0.
+  clear Hfindadd.
+  Info 1 auto.
+  inversion H0.
+  rewrite /connection_tree2expr //.
+Qed.
+
+Lemma expandBranch_connection_when_match :
+  forall c s1 s2 cm cm' cm'' cm0 tm tm' tm'' tm0 (seq_result : HiFP.hfstmt_seq),
+  cm' = (snd (expandBranch_funs s1 (Some seq_result) cm)) ->
+  cm'' = (snd (expandBranch_funs s2 (Some seq_result) cm)) ->
+  tm' = (expandBranch_connection_trees s1 tm) ->
+  tm'' = (expandBranch_connection_trees s2 tm) ->
+  (forall v texpr1 ttree1,
+  CEP.find v cm' = texpr1 ->
+  CEP.find v tm' = Some ttree1 ->
+  texpr1 = connection_tree2expr ttree1) ->
+  (forall v texpr2 ttree2,
+  CEP.find v cm'' = texpr2 ->
+  CEP.find v tm'' = Some ttree2 ->
+  texpr2 = connection_tree2expr ttree2) ->
+  expandBranch_connection_stmts s1 cm cm' tm tm' ->
+  expandBranch_connection_stmts s2 cm cm'' tm tm'' ->
+  expandBranch_connection_stmt (Swhen c s1 s2) cm cm0 tm tm0.
+Proof.
+  intros.
+  apply ExpandBranch_connection_when with (cm' := cm') (cm'' := cm'') (tm' := tm') (tm'' := tm''); try by done.
+  intros.
+  specialize H3 with (v := v) (texpr1 := texpr1) (ttree1 := ttree1).
+  specialize H4 with (v := v) (texpr2 := texpr2) (ttree2 := ttree2).
+  rewrite H3; try by done.
+  rewrite H4; try by done.
+  clear H3 H4 H8 H9 H10 H11.
+  move : H12.
+  case Ht1 : ttree1 => [||e1|c1 tt1 ft1].
+    - (* T_undefined *)
+    admit.
+    - (* T_invalid *)
+    admit.
+    - (* T_expr *)
+    case Ht2 : ttree2 => [||e2|c2 tt2 ft2].
+      - (* T_undefined *)
+      admit.
+      - (* T_invalid *)
+      admit.
+      - (* T_expr *)
+      simpl.
+      move => Hchoice.
+      inversion Hchoice.
+      clear H4 Hchoice.
+      simpl.
+      done.
+      - (* T_choice *)
+      move => Hchoice.
+      simpl in Hchoice.
+      inversion Hchoice.
+      clear H4 Hchoice.
+      rewrite {1}/connection_tree2expr.
+      case Hsn: (connection_tree2expr (T_choice c2 tt2 ft2)) => [texpr|]; try by done.
+      case Htexpr: texpr => [||te]; try by done.
+      rewrite Htexpr in Hsn.
+      admit.
+      admit.
+      admit.
+      admit. 
+    - (* T_choice *)
+    case Hsn1: (connection_tree2expr (T_choice c1 tt1 ft1)) => [texpr|]; try by done.
+    case Htexpr1: texpr => [||te]; try by done.
+    rewrite Htexpr1 in Hsn1.
+    admit. (* undefined *)
+
+    case Ht2 : ttree2 => [||e2|c2 tt2 ft2].
+      - (* T_undefined *)
+      simpl.
+      move => Hchoice.
+      inversion Hchoice.
+      clear H4 Hchoice.
+      rewrite Hsn1 Htexpr1//.
+      - (* T_invalid *)
+      simpl.
+      move => Hchoice.
+      inversion Hchoice.
+      clear H4 Hchoice.
+      rewrite Hsn1 Htexpr1//.
+      - (* T_expr *)
+      rewrite {1}/connection_tree2expr.
+      simpl.
+      move => Hchoice.
+      inversion Hchoice.
+      rewrite Htexpr1 in Hsn1.
+      clear H4 Hchoice.
+      admit.
+      - (* T_choice *)
+      case Hsn2: (connection_tree2expr (T_choice c2 tt2 ft2)) => [texpr'|]; try by done.
+      case Htexpr2: texpr' => [||te']; try by done.
+      rewrite Htexpr2 in Hsn2.
+        (* undefined *)
+        admit.
+        (* invalid *)
+        rewrite Htexpr1 in Hsn1.
+        rewrite Htexpr2 in Hsn2.
+        simpl.
+        admit.
+        (* expr *)
+        rewrite Htexpr1 in Hsn1.
+        rewrite Htexpr2 in Hsn2.
+        simpl.
+        admit.
+        (* None *)
+        admit.
+    case Ht2 : ttree2 => [||e2|c2 tt2 ft2].
+      - (* T_undefined *)
+      simpl.
+      move => Hchoice.
+      inversion Hchoice.
+      clear H4 Hchoice.
+      rewrite Hsn1 Htexpr1//.
+      - (* T_invalid *)
+      simpl.
+      move => Hchoice.
+      inversion Hchoice.
+      clear H4 Hchoice.
+      rewrite Hsn1 Htexpr1//.
+      - (* T_expr *)
+      rewrite {1}/connection_tree2expr.
+      simpl.
+      move => Hchoice.
+      inversion Hchoice.
+      rewrite Htexpr1 in Hsn1.
+      clear H4 Hchoice.
+      admit.
+      - (* T_choice *)
+      case Hsn2: (connection_tree2expr (T_choice c2 tt2 ft2)) => [texpr'|]; try by done.
+      case Htexpr2: texpr' => [||te']; try by done.
+      rewrite Htexpr2 in Hsn2.
+        (* undefined *)
+        admit.
+        (* invalid *)
+        rewrite Htexpr1 in Hsn1.
+        rewrite Htexpr2 in Hsn2.
+        simpl.
+        admit.
+        (* expr *)
+        rewrite Htexpr1 in Hsn1.
+        rewrite Htexpr2 in Hsn2.
+        simpl.
+        admit.
+        (* None *)
+        admit.
+    (* None *)
+    admit.
+Admitted.
+*)
+
+Lemma expandBranch_connection_when_match' : 
+  forall c s1 s2 cm cm0 tm tm0 (seq_result : HiFP.hfstmt_seq),
+  texpr_match_ttree cm tm ->
+  cm0 = (snd (expandBranch_fun (Swhen c s1 s2) (Some seq_result) cm)) ->
+  tm0 = (expandBranch_connection_tree (Swhen c s1 s2) tm) ->
+  expandBranch_connection_stmt (Swhen c s1 s2) cm cm0 tm tm0.
+Proof.
+  move => c s1 s2 cm cm0 tm tm0 seq_result Hpre Hcm0 Htm0.
+  apply ExpandBranch_connection_when; try by done.
+  simpl in Hcm0.
+  simpl in Htm0.
+  assert (Hm1 : texpr_match_ttree ((expandBranch_funs s1 (Some seq_result) cm).2) (expandBranch_connection_trees s1 tm)).
+  admit. (* 从stmts match可得 *)
+  assert (Hm2 : texpr_match_ttree ((expandBranch_funs s2 (expandBranch_funs s1 (Some seq_result) cm).1 cm).2) ((expandBranch_connection_trees s2 tm))).
+  admit.
+  rewrite /texpr_match_ttree.
+  rewrite Hcm0 Htm0.
+  clear Hcm0 Htm0.
+  move => v texpr0 ttree0 Hexpr0 Htree0.
+  rewrite StructStateP.Lemmas.map2_1bis in Hexpr0.
+  rewrite StructStateP.Lemmas.map2_1bis in Htree0.
+  case Ht1 : (CEP.find v (expandBranch_connection_trees s1 tm)).
+
+
+  (*rewrite /texpr_match_ttree in Hm1.
+  rewrite /texpr_match_ttree in Hm2.*)
+
+  admit.
+  1,2: simpl.
+  1,2: done.
+
+Qed.
+
+
+Lemma expandBranch_connection_stmt_match (s : HiFP.hfstmt) :
+  forall cm cm' tm tm' (seq_result : HiFP.hfstmt_seq),
+  texpr_match_ttree cm tm ->
+  cm' = snd (expandBranch_fun s (Some seq_result) cm) ->
+  tm' = expandBranch_connection_tree s tm ->
+  expandBranch_connection_stmt s cm cm' tm tm'
+with expandBranch_connection_stmts_match (ss : HiFP.hfstmt_seq) :
+  forall cm cm' tm tm' (seq_result : HiFP.hfstmt_seq),
+  texpr_match_ttree cm tm ->
+  cm' = snd (expandBranch_funs ss (Some seq_result) cm) ->
+  tm' = expandBranch_connection_trees ss tm ->
+  expandBranch_connection_stmts ss cm cm' tm tm'.
+Proof.
+  clear expandBranch_connection_stmt_match.
+  case Hs : s => [|v t|||||||c s1 s2]; try done.
+  - move => cm cm' tm tm' seq_result Hpre Hcm' Htm'.
+    simpl in Hcm'.
+    simpl in Htm'.
+    rewrite Hcm' Htm'.
+    apply ExpandBranch_connection_skip.
+  - 
+  admit.
+  admit.
+  admit.
+  admit.
+  admit.
+  admit.
+  admit.
+  - (* when *)
+  admit.
+
+  clear expandBranch_connection_stmts_match.
+
+  induction ss.
+  - move => cm cm' tm tm' seq_result Hpre Hcm' Htm'.
+    simpl in Hcm'.
+    simpl in Htm'.
+    rewrite Hcm' Htm'.
+    apply ExpandBranch_connections_nil.
+  - move => cm cm' tm tm' seq_result Hpre Hcm' Htm'.
+    simpl in Hcm'.
+    simpl in Htm'.
+    apply ExpandBranch_connections_con with (cm' := snd (expandBranch_fun h (Some seq_result) cm)) (tm' := (expandBranch_connection_tree h tm)).
+    apply expandBranch_connection_stmt_match with (seq_result := seq_result); try by done.
+    case Hf : ((expandBranch_fun h (Some seq_result) cm).1) => [seq_result'|].
+    rewrite Hf in Hcm'.
+    apply IHss with (seq_result := seq_result'); try by done.
+    admit. (* same as 单条 *)
+    admit. (* (expandBranch_fun h (Some seq_result) cm).1 = None *)
+Admitted.
+
+(* old version
+Definition ExpandBranch_connection_match (ss : HiFP.hfstmt_seq) : Prop :=
+ forall (v : pvar) (ce_other_modules : CEP.env) (cm_init : CEP.t def_expr) (init_decl_map : CEP.env) (ce : CEP.env),
+ match (CEP.find v (expandBranch_connection_tree ss (CEP.empty expr_tree))) with
+ | None => True (* ? *)
+ | Some expr_tree => CEP.find v (snd (expandBranch_fun ss ce_other_modules (Qnil ProdVarOrder.T) cm_init))
+ = connection_tree2expr expr_tree
+end.
+
+(*Lemma expandBranch_connection_stmt_match (s : HiFP.hfstmt) :
+  forall cm cm' tm tm' (seq_result : HiFP.hfstmt_seq),
+  cm' = snd (expandBranch_fun s (Some seq_result) cm) ->
+  tm' = expandBranch_connection_tree s tm ->
+  expandBranch_connection_stmt s cm cm' tm tm'
+with expandBranch_connection_stmts_match (ss : HiFP.hfstmt_seq) :
+  forall cm cm' tm tm' (seq_result : HiFP.hfstmt_seq),
+  cm' = snd (expandBranch_funs ss (Some seq_result) cm) ->
+  tm' = expandBranch_connection_trees ss tm ->
+  expandBranch_connection_stmts ss cm cm' tm tm'.
+Proof.
+  clear expandBranch_connection_stmt_match.
+      case Hh : h => [|v t|v r|v m|v1 v2|v e|v e|v|e s1 s2].
+    - (* skip *)
+      apply ExpandBranch_connection_skip.
+    - (* wire *)
+    case Hf : (CEP.find v (expandBranch_connection_tree (Swire v t) tm)) => [e|].
+    apply expandBranch_connection_wire_match with (texpr := (CEP.find v (snd (expandBranch_fun (Swire v t) (Some seq_result) cm))))  (ttree := e).
+    done.
+    rewrite Hf //.
+    assert (CEP.mem v (expandBranch_connection_tree (Swire v t) tm)).
+    simpl.
+    rewrite HiFP.PCELemmas.mem_add_eq //.
+    apply CEP.SE.eq_refl.
+    simpl in Hf.
+    rewrite HiFP.PCELemmas.add_eq_o in Hf.
+    discriminate.
+    apply CEP.SE.eq_refl.
+      (* reg *)
+      admit.
+      admit.
+      admit.
+      admit.
+      admit.
+      admit.
+    (* when *)
+    apply expandBranch_connection_when_match with (cm' := (snd (expandBranch_funs s1 (Some seq_result) cm)))
+      (cm'' := (snd (expandBranch_funs s2 (Some seq_result) cm))) (tm' := (expandBranch_connection_trees s1 tm)) 
+      (tm'' := (expandBranch_connection_trees s2 tm)) (seq_result := seq_result); try by done.
+    admit.
+    admit.
+    admit.
+    admit.
+
+    case Hf : (fst (expandBranch_fun h (Some seq_result) cm)) => [seq_result'|].
+    specialize IHss with (cm := snd (expandBranch_fun h (Some seq_result) cm)) (cm' := cm') 
+    (tm := (expandBranch_connection_tree h tm)) (tm' := tm') (seq_result := seq_result').
+    apply IHss; try by done.
+    rewrite H. 
+    clear H H0.
+    move : IHss.
+    case Hh :( expandBranch_fun h (Some seq_result) cm) => [t1 t2].
+    move => IHss.
+    rewrite -Hf Hh.
+    simpl.
+    done.
+
+    (* (expandBranch_fun h (Some seq_result) cm).1 = None
+    discriminate. *)
+
+Fixpoint already_ground_type (ss : HiFP.hfstmt_seq) (prop : Prop) : Prop :=
+  match ss with
+  | Qnil => prop
+  | Qcons s st => let new_prop := (match s with
+                  | Sskip => prop
+                  | Swire _ ty => match ty with
+                                  | Gtyp _ => prop
+                                  | _ => False
+                                  end
+                  | Sreg r reg => match (type reg) with
+                                  | Gtyp _ => prop
+                                  | _ => False
+                                  end
+                  | Smem r mem => match (data_type mem) with
+                                  | Gtyp _ => prop
+                                  | _ => False
+                                  end
+                  | Swhen _ s1 s2 => already_ground_type s1 prop /\ already_ground_type s2 prop
+                  | _ => prop
+                  end) 
+                  in already_ground_type st new_prop
+  end.
+
+Lemma add_expandBranch_connection : 
+  forall (ss : HiFP.hfstmt_seq) (ce_other_modules : CEP.env) (result : HiFP.hfstmt_seq) (cm_init : CEP.t def_expr)
+  (v r : pvar) (texpr : def_expr),
+  if v == r then CEP.find v (snd (expandBranch_fun ss ce_other_modules result (CEP.add r texpr cm_init))) = Some texpr
+  else CEP.find v (snd (expandBranch_fun ss ce_other_modules result (CEP.add r texpr cm_init))) = CEP.find v (snd (expandBranch_fun ss ce_other_modules result cm_init)).
+Proof.
+Admitted.
+
+Lemma add_expandBranch_connection_tree :
+  forall (ss : HiFP.hfstmt_seq) (v r : pvar) (tchild : expr_tree),
+  if v == r then CEP.find v
+    (expandBranch_connection_tree ss
+      (CEP.add r T_undefined (CEP.empty expr_tree))) = Some T_undefined
+  else (expandBranch_connection_tree ss (CEP.add r T_undefined (CEP.empty expr_tree))) = (expandBranch_connection_tree ss (CEP.empty expr_tree)).
+Proof.
+Admitted.
+
+Theorem ExpandWhens_connection_correct :
+  forall (ss : HiFP.hfstmt_seq),
+  already_ground_type ss True -> ExpandBranch_connection_match ss
+with ExpandWhens_connection_correct_Swhen :
+  forall (s : HiFP.hfstmt),
+  match s with
+  | Swhen c ss_true ss_false => already_ground_type ss_true True ->
+                                already_ground_type ss_false True ->
+                                ExpandBranch_connection_match ss_true /\
+                                ExpandBranch_connection_match ss_false
+  | _ => True
+  end.
+Proof.
+  (* prove ExpandWhens_connection_correct *)
+  clear ExpandWhens_connection_correct.
+  intros.
+  induction ss. 
+  - rewrite /ExpandBranch_connection_match.
+    simpl.
+    trivial.
+  - rewrite /ExpandBranch_connection_match.
+    intros.
+    rewrite /ExpandBranch_connection_match in IHss.
+    case Htree : (CEP.find v (expandBranch_connection_tree (Qcons h ss) (CEP.empty expr_tree))) => [t|]; try done.
+    unfold expandBranch_connection_tree in Htree; fold expandBranch_connection_tree in Htree.
+    unfold expandBranch_fun; fold expandBranch_fun.
+    move : t Htree.
+    case Hh : h => [|r ty|r reg||||||c ts fs]; try done.
+      - (* skip *)
+      intros.
+      specialize IHss with (v := v) (ce_other_modules := ce_other_modules) (cm_init := cm_init).
+      rewrite Htree in IHss.
+      simpl in H. 
+      rewrite Hh in H.
+      rewrite IHss //.
+      - (* wire *)
+      intros.
+      rewrite /init_ref.
+      simpl in H. 
+      rewrite Hh in H.
+      move : H.
+      case ty => [gt||]; try done.
+        - (* ground type *)
+        move => Hground.
+        case Heq : (v == r).
+        specialize add_expandBranch_connection with (ss := ss) (ce_other_modules := ce_other_modules)
+          (result := (Qcons (Swire (var:=ProdVarOrder.T) r (Gtyp gt)) (Qnil ProdVarOrder.T))) (cm_init := cm_init) (v := v) (r := r) (texpr := D_undefined).
+        move => Hadd.
+        rewrite Heq in Hadd.
+        rewrite Hadd.
+        rewrite /connection_tree2expr.
+        
+  admit.
+  (* prove ExpandWhens_connection_correct_Swhen *)
+  clear ExpandWhens_connection_correct_Swhen.
+  intro.
+  destruct s; try done.
+  intros.
+  split.
+  apply ExpandWhens_connection_correct.
+  done.
+  apply ExpandWhens_connection_correct.
+  done.
+Admitted.
+*)*)
+
+
+
+End ExpandWhens.
